Added specifications for buftxn read/write

src/program_proof/buftxn/idealized_buftxn_spec.v
@@ -3,18 +3,27 @@ From Perennial.algebra Require Import auth_map.
 From Goose.github_com.mit_pdos.goose_nfsd Require Import buftxn.
 From Perennial.program_proof Require Import buf.buf_proof addr.addr_proof.
 From Perennial.program_proof Require Import proof_prelude.
+From Perennial.goose_lang.lib Require Import slice.typed_slice.
 From Perennial.goose_lang.ffi Require Import disk_prelude.
 
-Notation bufDataDyn := {K & bufDataT K}.
+(* an object is the data for a sub-block object, a dynamic bundle of a kind and
+data of the appropriate size *)
+(* NOTE(tej): not necessarily the best name, because it's so general as to be
+meaningless *)
+Notation object := {K & bufDataT K}.
+
+Definition objKind (obj: object): bufDataKind := projT1 obj.
+Definition objData (obj: object): bufDataT (objKind obj) := projT2 obj.
 
 Class buftxnG Σ :=
-  { buftxn_buffer_inG :> mapG Σ addr bufDataDyn; }.
+  { buftxn_buffer_inG :> mapG Σ addr object; }.
 
 Section goose_lang.
   Context `{!heapG Σ}.
   Context `{!buftxnG Σ}.
 
   Implicit Types (l: loc) (γtxn γ: gname).
+  Implicit Types (obj: object).
 
   (* this is for the entire txn manager, and relates it to some ghost state *)
   Definition is_txn l γtxn : iProp Σ.
@@ -23,36 +32,74 @@ Section goose_lang.
   (* TODO: this is complicated - it needs to assert ownership over a block in
   the transaction system's abstract state (by instantiating the HOCAP P with
   some auth state) but actually only assert ownership over a sub-block *)
-  Definition stable_maps_to γtxn (a: addr) (data: bufDataDyn): iProp Σ.
+  Definition stable_maps_to γtxn (a: addr) obj: iProp Σ.
   Admitted.
 
   (* TODO: name this better *)
   Definition buftxn_ctx γ (bufs: gmap addr buf) : iProp Σ :=
-    ∃ (owned_bufs: gmap addr bufDataDyn),
+    ∃ (owned_bufs: gmap addr object),
       (* NOTE: this data is a superset of what's actually in the buftxn; can do
       an update to move ownership of an address into the transaction, which
       makes it available for reading (actually materializing the value) and
       writing (including overwrites without reading) *)
-      ⌜(λ bf, existT bf.(bufKind) bf.(bufData)) <$> bufs ⊆ owned_bufs⌝ ∗
-      map_ctx γ owned_bufs.
+      "%Hown_super" ∷ ⌜(λ bf, existT bf.(bufKind) bf.(bufData)) <$> bufs ⊆ owned_bufs⌝ ∗
+      "Howned●" ∷ map_ctx γ owned_bufs.
 
   (* this is for a single buftxn (transaction) - not persistent, buftxn's are
   not shareable *)
   Definition is_buftxn l (γtxn γ: gname) : iProp Σ :=
     ∃ (txn_l: loc) (bufs_l: loc) (bufs: gmap addr buf),
-      readonly (l ↦[BufTxn.S :: "txn"] #txn_l) ∗
-      readonly (l ↦[BufTxn.S :: "bufs"] #bufs_l) ∗
-      is_txn txn_l γtxn ∗
-      is_bufmap bufs_l bufs ∗
-      buftxn_ctx γ bufs.
+      "txn" ∷ readonly (l ↦[BufTxn.S :: "txn"] #txn_l) ∗
+      "bufs" ∷ readonly (l ↦[BufTxn.S :: "bufs"] #bufs_l) ∗
+      "Htxn" ∷ is_txn txn_l γtxn ∗
+      "Hbufs" ∷ is_bufmap bufs_l bufs ∗
+      "Hctx" ∷ buftxn_ctx γ bufs.
 
-  Definition buftxn_maps_to γtxn γ (a: addr) (data: bufDataDyn): iProp Σ :=
-    ptsto γ a 1 data ∗
-    ∃ data0, stable_maps_to γtxn a data0.
+  Definition buftxn_maps_to γtxn γ (a: addr) obj : iProp Σ :=
+    (∃ q, ptsto γ a q obj) ∗
+    ∃ obj0, stable_maps_to γtxn a obj0 ∗
+             ptsto γ a 1 obj.
 
-  Theorem lift_into_txn γtxn γ bufs a data :
-    buftxn_ctx γ bufs ∗ stable_maps_to γtxn a data  ==∗
-    buftxn_maps_to γtxn γ a data ∗ buftxn_ctx γ bufs.
-  Proof. Admitted.
+  Theorem lift_into_txn γtxn γ bufs a obj :
+    buftxn_ctx γ bufs -∗
+    stable_maps_to γtxn a obj ==∗
+    buftxn_maps_to γtxn γ a obj ∗ buftxn_ctx γ bufs.
+  Proof.
+    (* TODO: allocate into buftxn_ctx, consume stable_maps_to into
+    buftxn_maps_to *)
+  Admitted.
+
+  Definition is_object l a obj: iProp Σ :=
+    ∃ dirty, is_buf l a
+                    {| bufKind := objKind obj;
+                       bufData := objData obj;
+                       bufDirty := dirty |}.
+
+  Theorem wp_BufTxn__ReadBuf l γtxn γ (a: addr) (sz: u64) obj :
+    bufSz (objKind obj) = int.nat sz →
+    {{{ is_buftxn l γtxn γ ∗ buftxn_maps_to γtxn γ a obj }}}
+      BufTxn__ReadBuf #l (addr2val a) #sz
+    {{{ (l:loc), RET #l; is_object l a obj }}}.
+  Proof.
+  Admitted.
+
+  (* TODO: state that [data] (a slice of bytes in the implementation) encodes
+  the dynamically-typed object [obj], as *)
+  Definition data_has_obj (data: list byte) obj : Prop :=
+    match objData obj with
+    | bufBit _ => False (* TODO *)
+    | bufInode _ => False (* TODO *)
+    | bufBlock b => vec_to_list b = data
+    end.
+
+  Theorem wp_BufTxn__OverWrite l γtxn γ (a: addr) (sz: u64)
+          (data_s: Slice.t) q (data: list byte) obj0 obj :
+    bufSz (objKind obj) = int.nat sz →
+    data_has_obj data obj →
+    {{{ is_buftxn l γtxn γ ∗ buftxn_maps_to γtxn γ a obj0 ∗ is_slice data_s byteT q data }}}
+      BufTxn__OverWrite #l (addr2val a) (slice_val data_s)
+    {{{ RET #(); buftxn_maps_to γtxn γ a obj }}}.
+  Proof.
+  Admitted.
 
 End goose_lang.
